Added Database.fst
Made some changes in the protocol

Code/IdentityProvider.fst
@@ -5,8 +5,18 @@ open Crypto
 (* Must handle a receivesaml from authentication provider that specifies the second
 authentication method and then prompt client for it - and handle if the clients
 information was correct *)
+
+type SecurityRestriction = 
+	| Session: 1
+	| User: 2
+	| IdP: 4
+
+type SecurityProfile =
+	| Profile:	prin -> SecurityRestriction ->
+				int -> SecurityProfile
+
 val identityprovider: me:prin -> user:prin -> authp:prin -> unit
-val authenticateuser: me:prin -> authp:prin -> unit
+val authenticateuser: me:prin -> user:prin -> authp:prin -> unit
 
 let rec identityprovider me user authp =
 	let request = ReceiveSaml user in
@@ -24,29 +34,26 @@ let rec identityprovider me user authp =
 		let sigIdP = Sign me myprivk authnReq in
 		let req = AuthnRequestMessage me authp authnReq loginInfo sigIdP in
 		SendSaml authp req;
-		identityprovider me client authp
+		identityprovider me user authp
+	| 
+	| _ -> SendSaml user (DisplayError 400);
+		identityprovider me user authp
 
-	| AuthResponseMessage (issuer, destination, encassertion) ->
+let rec authenticateuser me user authp =
+	let request = ReceiveSaml authp in
+	match request with
+	| AuthResponseMessage(issuer, destination, encassertion, authmethod) ->
 		let meprivk = CertStore.GetPrivateKey me in
 		let assertion = DecryptAssertion me meprivk encassertion in
 		match assertion with
 		| SignedAssertion (token, sigAuthP) ->
-			let issuerpubkey = CertStore.GetPublicKey authp in
-			if VerifySignature authp issuerpubkey token sigAuthP
-			then 
+			let pubkissuer = CertStore.GetPublicKey authp in
+			if VerifySignature authp pubkissuer token sigAuthP
+			then
 				(assert (Log authp token);
-				let response = LoginResponse "You are now logged in" in
-				SendSaml client response)
-			else SendSaml client (DisplayError 403);
-			identityprovider me user authp
-	| _ -> SendSaml client (DisplayError 400);
-		identityprovider me user authp
-
-let rec authenticateuser me authp =
-	let request = ReceiveSaml authp in
-	match request with
-	| UserAuthenticated(...) ->
-		let flot = 
-		SendSaml client (*information about the n-factor auth*)
-		authenticateuser me authp
-	| _ -> SendSaml client (DisplayError 400);
+				let response = UserAuthRequest authmethod request in
+				SendSaml user response)
+			else SendSaml user (DisplayError 403);
+			authenticateuser me user authp
+	| _ -> SendSaml user (DisplayError 400);
+		authenticateuser me user authp
