Code/AuthenticationProvider.fst
@@ -2,25 +2,49 @@ module Authenticationprovider
 
 open SamlProtocol
 open Crpyto
+open Database
 (*Must send saml to identity provider about the ways of second
 authentication method and what is the correct information.
 Perhaps via the client. No contact to the client in this? Only IdP?*)
 val authenticationprovider me:prin -> idp:prin -> unit
-let authenticationprovider me idp =
+let rec authenticationprovider me idp =
 	let req = ReceiveSaml idp in
 	match req with
 	| AuthnRequestMessage (issuer, destination, message, loginInfo, sigIdP) ->
 		let pubkissuer = CertStore.GetPublicKey issuer in
 		(*Add check for the blacklist / whitelist in db in the if statement before
 		verifysignature*)
-		if (VerifySignature issuer pubkissuer message sigIdP) then
+		if (whitelisted idp && VerifySignature issuer pubkissuer message sigIdP) then
 			(assert (Log issuer message);
-			(*Check logindata vs the info stored in db*)
-			(*Send back information to idp about the n-factor auth*)
-			SendSaml idp (?);
-			authenticationprovider me idp
+			match loginInfo with
+			| CprLogin(cpr, password) ->
+				if(!cprrevokedidp cpr idp && checkcprlogin cpr password) then
+					(*Func for checking if this idp has been revoked by user*)
+					(*Func for checking the login info*)
+					(*Find the n-factor auth method - How / which one if more?*)
+					let authmethod = cprgetnfactor cpr in
+					SendSaml idp AuthResponseMessage authp idp Assertion(*?*) authmethod;
+					authenticationprovider me idp
+				else
+					SendSaml idp (LoginFailed);
+					authenticationprovider me idp
+			| UserLogin(name, password) ->
+				if(!revokedidp name idp && checkuserlogin name password) then
+					(*Func for checking if this idp has been revoked by user*)
+					(*Func for checking the login info*)
+					(*Find the n-factor auth method - How / which one if more?*)
+					let authmethod = getnfactor name in
+					SendSaml idp AuthResponseMessage authp idp Assertion(*?*) authmethod;
+					authenticationprovider me idp
+				else
+					SendSaml idp (LoginFailed);
+					authenticationprovider me idp
+			| _ -> SendSaml idp (Failed Requester);
+				authenticationprovider me idp
 		else
 			SendSaml idp (Failed Requester);
 			authenticationprovider me idp
 	| _ -> SendSaml idp (Failed Requester);
 		authenticationprovider me idp
+
+(*Add database func*)
