Code/Database.fst
@@ -1,0 +1,31 @@
+module Database
+
+open SamlProtocol
+open Crypto
+
+(*Identity provider functionality*)
+val whitelist: idp:prin -> unit
+val blacklist: idp:prin -> unit
+val addidp: idp:prin -> unit
+val whitelisted: idp:prin -> bool
+
+(*User functionality*)
+val adduser: user:string -> password:string -> unit
+val addcpruser: cpr:int -> password:string -> unit
+
+val addnfactor: user:string -> nfactor:Authentication -> unit
+val removenfactor: user:string -> nfactor:Authentication -> unit
+val cpraddnfactor: cpr:int -> nfactor:Authentication -> unit
+val cprremovenfactor: cpr:int -> nfactor:Authentication -> unit
+
+val getnfactor: user:string -> Authentication
+val cprgetnfactor: cpr:int -> Authentication
+
+val checkcprlogin: cpr:int -> password:string -> bool
+val checkuserlogin: user:string -> password:string -> bool
+
+val revokeidp: cpr:int -> idp:prin -> unit
+val revokeidp: user:string -> idp:prin -> unit
+
+val revokedidp: user:string -> idp:prin -> bool
+val cprrevokedidp: cpr:int -> idp:prin -> bool
